redesign of have @ and hide
git-svn-id: svn+ssh://scm.gforge.inria.fr/svnroot/coqfinitgroup/trunk@4650 305884b8-be16-0410-aa53-a3be2363cef1

ssreflect.v
@@ -352,7 +352,7 @@ Proof. exact: unlock. Qed.
 Definition ssr_have Plemma Pgoal (step : Plemma) rest : Pgoal := rest step.
 Implicit Arguments ssr_have [Pgoal].
 
-Definition ssr_have_let Plemma step Pgoal
+Definition ssr_have_let Pgoal Plemma step
   (rest : let x : Plemma := step in Pgoal) : Pgoal := rest.
 Implicit Arguments ssr_have_let [Pgoal].
 
@@ -409,3 +409,17 @@ Definition ssrhidden (T : Type) (t : T) : T := t.
 Notation "<hidden>" := (ssrhidden _) (at level 0).
 Definition ssrhiddenas (T1 : Type) (t1 : T1) (T2 : Type) (t2 : T2) : T1 := t1.
 Notation "<hidden X >" := (ssrhiddenas _ X) (at level 0, format "<hidden  X >").
+
+(* Canonical names for unit and tt *)
+Definition skolem_lock := unit.
+Definition skolem_key := tt.
+
+Definition skolem (statement : Type) (skolem_id : nat) (lock : skolem_lock) :=
+  let: tt := lock in statement.
+
+Lemma use_skolem T n l (x : skolem T n l) : T.
+Proof. by case: l x. Qed.
+
+Notation "<skolem n >" := (skolem _ n _).
+Notation "( T )" := (skolem T _ skolem_key).
+
